FY/Grover.v
@@ -10,33 +10,7 @@ From FY Require Export Logic.
 Definition X : string := "X".
 Definition Y0 : string := "Y0".
 Definition Y1 : string := "Y1".
-Definition Y2 : string := "Y2".
 Definition K : string := "K".
-
-Definition U100 : Matrix 8 8 := l2M [[1;0;0;0;0;0;0;0];
-                                     [0;1;0;0;0;0;0;0];
-                                     [0;0;1;0;0;0;0;0];
-                                     [0;0;0;-1%C;0;0;0;0];
-                                     [0;0;0;0;1;0;0;0];
-                                     [0;0;0;0;0;1;0;0];
-                                     [0;0;0;0;0;0;1;0];
-                                     [0;0;0;0;0;0;0;1]].
-
-Lemma U100W: U100 × ∣1,0,0⟩ == -1 * ∣1,0,0⟩.
-Proof.
-Admitted.
-
-(*TODO: not complete*)
-Lemma U100NW: forall (w: Vector 8), w <> ∣1,0,0⟩ -> U100 × w = w.
-Proof.
-Admitted.
-
-(* Definition G := GOracle 8 (( 2 * (∣+⟩⊗∣+⟩⊗∣+⟩⟨+∣⊗⟨+∣⊗⟨+∣) - (I 8)) × U100). *)
-
-
-(* Definition Us : Unitary 8 := ((∣+⟩⊗∣+⟩⊗∣+⟩)×(⟨+∣⊗⟨+∣⊗⟨+∣)) + (-1 * (I 8)). *)
-
-(* Definition G := GOracle 8 (Us × U100). *)
 
 Lemma kron_I_1: kron (I 2) (I 1) == I 2.
 Proof.
@@ -47,32 +21,61 @@ Definition GROVER : com :=
   <{
     new_qubit;
     new_qubit;
-    new_qubit;
     q 0 *= GH;
     q 1 *= GH;
-    q 2 *= GH;
-    K := (3 % nat); (* 3 ~ sqrt(8) *)
+    (*Oracle - start*)
+    q 0 *= GH;
+    q 1 *= GH;
+    q 0 *= GZ;
+    q 1 *= GZ;
+    (*Oracle - end*)
+    K := (2 % nat); (* 3 ~ sqrt(8) *)
     X := (0 % nat);
     while X <= K do
       q 0 1 *= GCNOT;
       X := (X + 1%nat)
     end;
     Y0 :=meas 0;
-    Y1 :=meas 1;
-    Y2 :=meas 2
+    Y1 :=meas 1
   }>.
 
 Print GROVER.
 
-Theorem final_state: ceval 0%nat 3%nat GROVER [(( _ !-> 0%nat), I 1)] [(( X !-> 3%nat ; K !-> 3%nat ; Y0 !-> 0%nat ; Y1 !-> 0%nat ;Y2 !-> 1%nat; _ !-> 0%nat), ∣0⟩⟨0∣ )] .
+Theorem final_state: ceval 0%nat 3%nat GROVER [(( _ !-> 0%nat), I 1)] 
+[(( X !-> 2%nat ; K !-> 2%nat ; 
+    Y0 !-> 0%nat ;
+    Y1 !-> 0%nat ; _ !-> 0%nat), ∣0⟩⟨0∣ )] .
 Proof.
   eapply E_Seq.
   apply E_Init.
   eapply E_Seq.
   apply E_Init.
   eapply E_Seq.
-  apply E_Init.
+  apply E_AppOne.
   eapply E_Seq.
+  simpl.
+  apply E_AppOne.
+  eapply E_Seq.
+  simpl.
+  apply E_AppOne.
+  eapply E_Seq.
+  simpl.
+  apply E_AppOne.
+  eapply E_Seq.
+  simpl.
+  apply E_AppOne.
+  eapply E_Seq.
+  simpl.
+  apply E_AppOne.
+  eapply E_Seq.
+  simpl.
+  apply E_Ass.
+  eapply E_Seq.
+  simpl.
+  apply E_Ass.
+  eapply E_Seq.
+  simpl.
+  eapply E_WhileTrue.
   (* there is a problem *)
 Admitted.
 
