FY/CoinToss.v
@@ -1,0 +1,98 @@
+From Coq Require Import Strings.String.
+From Coq Require Import Lists.List.
+Import ListNotations.
+From FY Require Export Utils.
+From FY Require Export Syntax.
+From FY Require Export Semantics.
+From FY Require Export Assertion.
+From FY Require Export Logic.
+
+Definition X : string := "X".
+
+Definition Prog : com :=
+  <{ new_qubit;
+     q 0 *= GH;
+     X :=meas 0
+    }>.
+
+Print Prog.
+
+Fact calc_0: 0.5 * ∣0⟩⟨0∣ = ∣0⟩⟨0∣ × (H × ∣0⟩⟨0∣ × (H) †) × (∣0⟩⟨0∣)†.
+Proof. Admitted.
+
+Fact calc_1: 0.5 * ∣1⟩⟨1∣ = ∣1⟩⟨1∣ × (H × ∣0⟩⟨0∣ × (H) †) × (∣1⟩⟨1∣)†.
+Proof. Admitted.
+
+Theorem operational_sem: 
+  ceval 0%nat 1%nat Prog [(( _ !-> 0%nat), I 1)] 
+  [(( X !-> 0%nat; _ !-> 0%nat), 0.5 * ∣0⟩⟨0∣ );
+   (( X !-> 1%nat; _ !-> 0%nat), 0.5 * ∣1⟩⟨1∣ )].
+Proof.
+    eapply E_Seq.
+    apply E_Init.
+    simpl.
+    eapply E_Seq.
+    apply E_AppOne.
+    simpl.
+    rewrite calc_0.
+    rewrite calc_1.
+    eapply E_Meas.
+Qed.
+
+Definition pre : Assertion 0%nat := ((_ !-> 0%nat), (BTrue, I 1)).
+Definition post : Assertion 1%nat := ((_ !-> 0%nat), (<{ X == (0 % nat)}>, 0.5 * ∣0⟩⟨0∣)).
+
+Lemma pre_is_init_sub: pre = (init_sub 1 (AssertionOf 1%nat (StateOf pre) (PropOf pre) (∣0⟩⟨0∣))).
+Proof. Admitted.
+
+Lemma assrt_is_apply_sub: 
+(AssertionOf 1 (StateOf pre) (PropOf pre) ∣0⟩⟨0∣)
+= (apply_sub 1 (geval GH) 
+(AssertionOf 1 (StateOf pre) (PropOf pre) (H × ∣0⟩⟨0∣ × (H) †))) .
+Proof. Admitted.
+
+Theorem prog_correct: hoare_triple pre Prog post.
+Proof.
+    eapply fy_sequence.
+    rewrite pre_is_init_sub.
+    assert (H1: hoare_triple (init_sub 1%nat (StateOf pre, (PropOf pre, ∣0⟩⟨0∣))) 
+    <{ new_qubit }> (AssertionOf 1%nat (StateOf pre) (PropOf pre) ∣0⟩⟨0∣)).
+    apply fy_init.
+    apply H1.
+    eapply fy_sequence.
+    assert (H2: hoare_triple (apply_sub 1 (geval GH) 
+    (AssertionOf 1 (StateOf pre) (PropOf pre) (H × ∣0⟩⟨0∣ × (H) †))) 
+    <{ q 0 *= GH }> (AssertionOf 1 (StateOf pre) (PropOf pre) (Utils.H × ∣0⟩⟨0∣ × Utils.H†))).
+    apply fy_apply.
+    rewrite assrt_is_apply_sub.
+    apply H2.
+    eapply fy_weakness.
+    remember (AssertionOf 1%nat (_ !-> 0%nat)
+      <{ X == (0 % nat) }> (H × ∣0⟩⟨0∣ × (H) †)) as pm.
+    assert (H8: hoare_triple (conjunction 
+        (AssertPreMeas (AssertionOf 1%nat (_ !-> 0%nat)
+        <{ X == (0 % nat) }> (H × ∣0⟩⟨0∣ × (H) †)) X 0%nat 0%nat) 
+        (AssertPreMeas (AssertionOf 1%nat (_ !-> 0%nat)
+        <{ X == (0 % nat) }> (H × ∣0⟩⟨0∣ × (H) †)) X 1%nat 0%nat))  
+        <{ X :=meas 0 }> 
+        (AssertionOf 1%nat (_ !-> 0%nat)
+        <{ X == (0 % nat) }> (H × ∣0⟩⟨0∣ × (H) †))).
+    apply fy_measure.
+    apply H8.
+    intros.
+    unfold weaker, AssertionWithDensity, conjunction,
+     AssertPreMeas, AssertionOf.
+    simpl.
+    unfold PropOf, DensityOf, StateOf.
+    simpl.
+    induction st.
+    simpl.
+    lra.
+    simpl.
+    destruct (mergeMaps (fst a) (_ !-> 0%nat) X =? 0) eqn:bv1.
+    simpl.
+    admit.
+    admit.
+    admit.
+Admitted.
+ 
