FY/GHZ.v
@@ -160,10 +160,10 @@ Abort.
 
 
 (* TODO : Swap gate+no cloning*)
-Definition P (tm: total_map nat): Assertion 3 :=  (tm, (<{ true }>, I 1)).
-Definition Q (tm: total_map nat): Assertion 3 :=  (tm, (<{ X1 == X2 }>, I 3)).
+Definition P : Assertion 3 :=  (( _ !-> 0%nat), (<{ true }>, I 1)).
+Definition Q : Assertion 3 :=  (( _ !-> 0%nat), (<{ X1 == X2 }>, I 3)).
 
-Theorem ghz_equality_end: forall tm, hoare_triple 0 3 (P tm) GHZ (Q tm).
+Theorem ghz_equality_end: hoare_triple P GHZ Q.
 Proof.
   intros.
   eapply fy_sequence.
