FY/Soundness.v
@@ -1,0 +1,44 @@
+From Coq Require Import Strings.String.
+From Coq Require Import Lists.List.
+Import ListNotations.
+From FY Require Export Utils.
+From FY Require Export Syntax.
+From FY Require Export Semantics.
+From FY Require Export Assertion.
+From FY Require Export Logic.
+
+Inductive derivable (np nq: nat) : Assertion np -> com -> Assertion nq -> Type :=
+| H_Skip : forall P,
+    derivable P <{skip}> P
+| H_Asgn : forall Q V a,
+    derivable (Q [V ⊢> a]) <{X := a}> Q
+| H_Seq : forall P c Q d R,
+    derivable P c Q -> derivable Q d R -> derivable P <{c;d}> R
+| H_If : forall P Q b c1 c2,
+  derivable (fun st => P st ∧ bassn b st) c1 Q ->
+  derivable (fun st => P st ∧ ~(bassn b st)) c2 Q ->
+  derivable P <{if b then c1 else c2 end}> Q
+| H_While : forall P b c,
+  derivable (fun st => P st ∧ bassn b st) c P ->
+  derivable P <{while b do c end}> (fun st => P st ∧ ~ (bassn b st))
+| H_Consequence : forall (P Q P' Q' : Assertion) c,
+  derivable P' c Q' ->
+  (forall st, P st -> P' st) ->
+  (forall st, Q' st -> Q st) ->
+  derivable P c Q.
+
+Definition valid (P : Assertion) (c : com) (Q : Assertion) : Prop :=
+  forall st st',
+     st =[ c ]=> st' ->
+     P st ->
+     Q st'.
+
+Theorem logic_sound : forall P c Q,
+  derivable P c Q -> valid P c Q.
+Proof.
+Admitted.
+
+Theorem hoare_complete: forall P c Q,
+  valid P c Q -> derivable P c Q.
+Proof.
+Admitted.
