FY/Teleportation.v
@@ -41,80 +41,26 @@ Proof.
     apply E_Init.
     simpl.
     eapply E_Seq.
-    
-    (* there is a problem *)
+    apply E_AppOne.
+    simpl.
+    eapply E_Seq.
+    simpl.
+    apply E_Init.
+    simpl.
+    eapply E_Seq.
+    apply E_AppTwo.
+    simpl.
+    eapply E_Seq.
+    apply E_AppTwo.
+    simpl.
+    eapply E_Seq.
+    apply E_AppOne.
+    simpl.
+    eapply E_Seq.
+    apply E_Meas.
+    simpl.
+    eapply E_Seq.
+    apply E_Meas.
+    simpl.
 Admitted.
-
-
-(*
-import numpy as np
-H = 1/np.sqrt(2)*np.array([[1, 1],
-                           [1,-1]])
-CNOT = np.array([[1,0,0,0],
-                 [0,1,0,0],
-                 [0,0,0,1],
-                 [0,0,1,0]])
-
-I = np.eye(2)
-
-ket0 = np.array([1,0])
-ket1 = np.array([0,1])
-
-init = np.kron(ket0, np.kron(ket0, ket0)).reshape(-1,1)
-
-fst = init.dot(init.T) 
-#print(fst)
-
-u1 = np.kron(H, np.kron(I, I))
-snd = u1.dot(fst).dot(u1.T)
-#print(snd)
-
-u2 = np.kron(CNOT , I)
-thrd = u2.dot(snd).dot(u2.T)
-#print(thrd)
-
-u3 = np.kron(I , CNOT)
-frth = u3.dot(thrd).dot(u3.T)
-print(frth)
-
-m0 = np.kron(ket0, np.kron(I, I))
-fth0 = m0.dot(frth).dot(m0.T) / np.trace(m0.dot(frth).dot(m0.T))
-print(fth0)
-
-m1 = np.kron(ket1, np.kron(I, I))
-fth1 = m1.dot(frth).dot(m1.T) / np.trace(m1.dot(frth).dot(m1.T))
-print(fth1)
-
-m0 = np.kron(ket0, I)
-sxth00 = m0.dot(fth0).dot(m0.T) / np.trace(m0.dot(fth0).dot(m0.T))
-print(sxth00)
-sxth01 = m0.dot(fth1).dot(m0.T) / np.trace(m0.dot(fth1).dot(m0.T))
-print(sxth01)
-
-m1 = np.kron(ket1, I)
-sxth10 = m1.dot(fth0).dot(m1.T) / np.trace(m1.dot(fth0).dot(m1.T))
-print(sxth10)
-m1 = np.kron(ket1, I)
-sxth11 = m1.dot(fth1).dot(m1.T) / np.trace(m1.dot(fth1).dot(m1.T))
-print(sxth11)
-
-
-prop000 = np.kron(ket0, np.kron(ket0, ket0)).T.dot(frth).dot(np.kron(ket0, np.kron(ket0, ket0)))
-print(prop000)
-prop001 = np.kron(ket0, np.kron(ket0, ket1)).T.dot(frth).dot(np.kron(ket0, np.kron(ket0, ket1)))
-print(prop001)
-prop010 = np.kron(ket0, np.kron(ket1, ket0)).T.dot(frth).dot(np.kron(ket0, np.kron(ket1, ket0)))
-print(prop010)
-prop011 = np.kron(ket0, np.kron(ket1, ket1)).T.dot(frth).dot(np.kron(ket0, np.kron(ket1, ket1)))
-print(prop011)
-prop100 = np.kron(ket1, np.kron(ket0, ket0)).T.dot(frth).dot(np.kron(ket1, np.kron(ket0, ket0)))
-print(prop100)
-prop101 = np.kron(ket1, np.kron(ket0, ket1)).T.dot(frth).dot(np.kron(ket1, np.kron(ket0, ket1)))
-print(prop101)
-prop110 = np.kron(ket1, np.kron(ket1, ket0)).T.dot(frth).dot(np.kron(ket1, np.kron(ket1, ket0)))
-print(prop110)
-prop111 = np.kron(ket1, np.kron(ket1, ket1)).T.dot(frth).dot(np.kron(ket1, np.kron(ket1, ket1)))
-print(prop111)
-
-*)
 
